Manual merge with latest proof additions.
We completed the proof refactoring to improve verification
times by manually guiding the automation on the last stable
point where the proof passes correctly without timeouts. We
are now transferring the latest progress in the proof to the
now improved structure of the proof.

docs/sbft-formal-model/proof.dfy
@@ -29,6 +29,8 @@ module Proof {
   import opened SafetySpec
   import opened Library
 
+  type Message = Network.Message<Messages.Message>
+
   predicate IsHonestReplica(c:Constants, hostId:HostId) 
   {
     && c.WF()
@@ -283,6 +285,7 @@ module Proof {
   predicate Inv(c: Constants, v:Variables) {
     //&& PrePreparesCarrySameClientOpsForGivenSeqID(c, v)
     // Do not remove, lite invariant about internal honest Node invariants:
+    && v.WF(c)
     && AllReplicasLiteInv(c, v)
     && RecordedPreparesHaveValidSenderID(c, v)
     //&& SentPreparesMatchRecordedPrePrepareIfHostInSameView(c, v)
@@ -300,10 +303,11 @@ module Proof {
     && HonestReplicasLockOnCommitForGivenView(c, v)
     && CommitMsgsFromHonestSendersAgree(c, v)
     && RecordedCheckpointsRecvdCameFromNetwork(c, v)
+    && UnCommitableAgreesWithPrepare(c, v)
   }
 
   function sentPreparesForSeqID(c: Constants, v:Variables, view:nat, seqID:Messages.SequenceID,
-                                  operationWrapper:Messages.OperationWrapper) : set<Network.Message<Messages.Message>> 
+                                  operationWrapper:Messages.OperationWrapper) : set<Message> 
     requires v.WF(c)
   {
     set msg | && msg in v.network.sentMsgs 
@@ -323,7 +327,7 @@ module Proof {
   }
 
   lemma WlogCommitAgreement(c: Constants, v:Variables, v':Variables, step:Step,
-                            msg1:Network.Message<Messages.Message>, msg2:Network.Message<Messages.Message>)
+                            msg1:Message, msg2:Message)
     requires Inv(c, v)
     requires NextStep(c, v, v', step)
     requires msg1 in v'.network.sentMsgs 
@@ -709,6 +713,130 @@ module Proof {
     h_v.workingWindow.reveal_Shift();
   }
 
+  lemma TriviallyPreserveUnCommitableAgreesWithPrepare(c: Constants, v:Variables, v':Variables, step:Step, h_v:Replica.Variables, h_step:Replica.Step)
+    requires Inv(c, v)
+    requires || (&& HonestReplicaStepTaken(c, v, v', step, h_v, h_step) 
+                 && (|| h_step.SendPrePrepareStep?
+                     || h_step.RecvPrePrepareStep?
+                     || h_step.RecvPrepareStep?
+                     || h_step.RecvCommitStep?
+                     || h_step.DoCommitStep?
+                     || h_step.ExecuteStep?
+                     || h_step.SendCheckpointStep?
+                     || h_step.RecvCheckpointStep?
+                     || h_step.AdvanceWorkingWindowStep?
+                     || h_step.PerformStateTransferStep?
+                     || h_step.SendViewChangeMsgStep?
+                     || h_step.RecvViewChangeMsgStep?
+                     || h_step.SelectQuorumOfViewChangeMsgsStep?
+                     || h_step.SendNewViewMsgStep?
+                     || h_step.RecvNewViewMsgStep?
+                     || h_step.SendCommitStep?))
+             || (NextStep(c, v, v', step) && c.clusterConfig.IsFaultyReplica(step.id))
+             || (NextStep(c, v, v', step) &&  c.clusterConfig.IsClient(step.id))
+      ensures UnCommitableAgreesWithPrepare(c, v')
+    {
+      reveal_UnCommitableAgreesWithPrepare();
+      forall prepareMsg:Message,
+               priorView:nat,
+               priorOperationWrapper:Messages.OperationWrapper
+                    | && prepareMsg.payload.Prepare? 
+                      && priorView < prepareMsg.payload.view
+                      && c.clusterConfig.IsHonestReplica(prepareMsg.sender)
+                      && priorOperationWrapper != prepareMsg.payload.operationWrapper
+                      && prepareMsg in v'.network.sentMsgs
+                      ensures UnCommitableInView(c, v', prepareMsg.payload.seqID, priorView, priorOperationWrapper) {
+        assert UnCommitableInView(c, v, prepareMsg.payload.seqID, priorView, priorOperationWrapper);
+        assert ReplicasThatCanCommitInView(c, v', prepareMsg.payload.seqID, priorView, priorOperationWrapper) 
+            == ReplicasThatCanCommitInView(c, v, prepareMsg.payload.seqID, priorView, priorOperationWrapper);
+        // assert |ReplicasThatCanCommitInView(c, v', prepareMsg.payload.seqID, priorView, priorOperationWrapper)|
+        //     == |ReplicasThatCanCommitInView(c, v, prepareMsg.payload.seqID, priorView, priorOperationWrapper)|;
+      }
+    }
+
+  lemma HonestLeaveViewStepPreservesUnCommitableAgreesWithPrepare(c: Constants, v:Variables, v':Variables, step:Step, h_v:Replica.Variables, h_step:Replica.Step)
+    requires Inv(c, v)
+    requires HonestReplicaStepTaken(c, v, v', step, h_v, h_step)
+    requires h_step.LeaveViewStep?
+    ensures UnCommitableAgreesWithPrepare(c, v')
+  {
+    reveal_UnCommitableAgreesWithPrepare();
+    forall prepareMsg:Message,
+             priorView:nat,
+             priorOperationWrapper:Messages.OperationWrapper
+                  | && prepareMsg.payload.Prepare? 
+                    && priorView < prepareMsg.payload.view
+                    && c.clusterConfig.IsHonestReplica(prepareMsg.sender)
+                    && priorOperationWrapper != prepareMsg.payload.operationWrapper
+                    && prepareMsg in v'.network.sentMsgs
+                    ensures UnCommitableInView(c, v', prepareMsg.payload.seqID, priorView, priorOperationWrapper) {
+      assert UnCommitableInView(c, v, prepareMsg.payload.seqID, priorView, priorOperationWrapper);
+      // assert ReplicasThatCanCommitInView(c, v', prepareMsg.payload.seqID, priorView, priorOperationWrapper) 
+      //     <= ReplicasThatCanCommitInView(c, v, prepareMsg.payload.seqID, priorView, priorOperationWrapper);
+      // assert |ReplicasThatCanCommitInView(c, v', prepareMsg.payload.seqID, priorView, priorOperationWrapper)|
+      //     <= |ReplicasThatCanCommitInView(c, v, prepareMsg.payload.seqID, priorView, priorOperationWrapper)|;
+      Library.SubsetCardinality(ReplicasThatCanCommitInView(c, v', prepareMsg.payload.seqID, priorView, priorOperationWrapper), 
+                                ReplicasThatCanCommitInView(c, v, prepareMsg.payload.seqID, priorView, priorOperationWrapper));
+    }
+  }
+
+  lemma HonestSendPrepareStepPreservesUnCommitableAgreesWithPrepare(c: Constants, v:Variables, v':Variables, step:Step, h_v:Replica.Variables, h_step:Replica.Step)
+    requires Inv(c, v)
+    requires HonestReplicaStepTaken(c, v, v', step, h_v, h_step)
+    requires h_step.SendPrepareStep?
+    ensures UnCommitableAgreesWithPrepare(c, v')
+  {
+    ///
+    reveal_EveryCommitClientOpMatchesRecordedPrePrepare();
+    reveal_AllReplicasLiteInv();
+    reveal_RecordedPreparesHaveValidSenderID();
+    reveal_RecordedPrePreparesRecvdCameFromNetwork();
+    reveal_RecordedPreparesInAllHostsRecvdCameFromNetwork();
+    reveal_RecordedPreparesMatchHostView();
+    reveal_RecordedPreparesClientOpsMatchPrePrepare();
+    reveal_RecordedCommitsClientOpsMatchPrePrepare();
+    reveal_EverySentIntraViewMsgIsInWorkingWindowOrBefore();
+    reveal_EverySentIntraViewMsgIsForAViewLessOrEqualToSenderView();
+    reveal_EveryPrepareClientOpMatchesRecordedPrePrepare();
+    reveal_EveryCommitClientOpMatchesRecordedPrePrepare();
+    reveal_HonestReplicasLockOnPrepareForGivenView();
+    reveal_HonestReplicasLockOnCommitForGivenView();
+    reveal_CommitMsgsFromHonestSendersAgree();
+    reveal_RecordedCheckpointsRecvdCameFromNetwork();
+    reveal_HonestReplicasLockOnCommitForGivenView();
+    reveal_EveryCommitMsgIsSupportedByAQuorumOfPrepares();
+    h_v.workingWindow.reveal_Shift();
+    ///
+
+    // if (h_step.SendPrepareStep?) {
+    //   assume false;
+    // } else if (h_step.LeaveViewStep?) {
+    //   assume false;
+    // } else if (h_step.SendCommitStep?) {
+    //   assume false; 
+    // }
+
+    reveal_UnCommitableAgreesWithPrepare();
+    forall prepareMsg:Message,
+             priorView:nat,
+             priorOperationWrapper:Messages.OperationWrapper
+                  | && prepareMsg.payload.Prepare? 
+                    && priorView < prepareMsg.payload.view
+                    && c.clusterConfig.IsHonestReplica(prepareMsg.sender)
+                    && priorOperationWrapper != prepareMsg.payload.operationWrapper
+                    && prepareMsg in v'.network.sentMsgs
+                    ensures UnCommitableInView(c, v', prepareMsg.payload.seqID, priorView, priorOperationWrapper) {
+      assert UnCommitableInView(c, v, prepareMsg.payload.seqID, priorView, priorOperationWrapper);
+      assert ReplicasThatCanCommitInView(c, v', prepareMsg.payload.seqID, priorView, priorOperationWrapper) 
+          == ReplicasThatCanCommitInView(c, v, prepareMsg.payload.seqID, priorView, priorOperationWrapper);
+      assert |ReplicasThatCanCommitInView(c, v', prepareMsg.payload.seqID, priorView, priorOperationWrapper)|
+          == |ReplicasThatCanCommitInView(c, v, prepareMsg.payload.seqID, priorView, priorOperationWrapper)|;
+      // assert |ReplicasThatCanCommitInView(c, v, prepareMsg.payload.seqID, priorView, priorOperationWrapper)| < c.clusterConfig.AgreementQuorum();
+    }
+  }
+
+  /// End Of Case Splitting
+
   lemma QuorumOfPreparesInNetworkMonotonic(c: Constants, v:Variables, v':Variables, step:Step)
     requires NextStep(c, v, v', step)
     ensures (forall view, seqID, clientOp | QuorumOfPreparesInNetwork(c, v, view, seqID, clientOp)
@@ -721,6 +849,277 @@ module Proof {
       var senders' := Messages.sendersOf(sentPreparesForSeqID(c, v', view, seqID, clientOp));
       Library.SubsetCardinality(senders, senders');
     }
+  }
+
+  predicate AgreementQuorumOfMessages(c:Constants, msgs:set<Message>) {
+    && c.WF()
+    && |msgs| >= c.clusterConfig.AgreementQuorum()
+    && Messages.UniqueSenders(msgs)
+  }
+
+  predicate isCommitQuorum(c:Constants,
+                           v:Variables,
+                           view:nat,
+                           seqID:Messages.SequenceID,
+                           operationWrapper:Messages.OperationWrapper,
+                           sentCommits:set<Message>) 
+    requires v.WF(c)
+  {
+    && sentCommits <= v.network.sentMsgs
+    && AgreementQuorumOfMessages(c, sentCommits)
+    && (forall msg | msg in sentCommits
+                    :: && msg.payload.Commit?
+                       && msg.payload.view == view
+                       && msg.payload.seqID == seqID
+                       && msg.payload.operationWrapper == operationWrapper
+                       && msg.sender in getAllReplicas(c))
+  }
+
+  lemma UniqueSendersCardinality(msgs:set<Message>)
+    requires Messages.UniqueSenders(msgs)
+    ensures |Messages.sendersOf(msgs)| == |msgs|
+  {
+    Messages.reveal_UniqueSenders();
+    if |msgs| > 0 {
+      var m :| m in msgs;
+      var subMsgs := msgs - {m};
+      UniqueSendersCardinality(subMsgs);
+      assert Messages.sendersOf(msgs) == Messages.sendersOf(subMsgs) + {m.sender};
+    }
+  }
+
+  function ReplicasThatCanCommitInView(c:Constants,
+                               v:Variables,
+                               seqID:Messages.SequenceID,
+                               view:nat,
+                               operationWrapper:Messages.OperationWrapper)
+                               : set<HostIdentifiers.HostId>
+    requires v.WF(c)
+  {
+    var replicasSentCommit := set replica |
+                               && replica in getAllReplicas(c)
+                               && c.clusterConfig.IsHonestReplica(replica)
+                               && Network.Message(replica,
+                                                    Messages.Commit(view,
+                                                                    seqID,
+                                                                    operationWrapper)) in v.network.sentMsgs;
+    var inViewOrLower := set replica | && replica in getAllReplicas(c)
+                                       && c.clusterConfig.IsHonestReplica(replica)
+                                       && var h_c := c.hosts[replica].replicaConstants;
+                                       && var h_v := v.hosts[replica].replicaVariables;
+                                       && h_v.view <= view;
+    var faultyReplicas := set replica | && replica in getAllReplicas(c)
+                                        && c.clusterConfig.IsFaultyReplica(replica);
+    replicasSentCommit + inViewOrLower + faultyReplicas
+  }
+
+  predicate UnCommitableInView(c:Constants,
+                               v:Variables,
+                               seqID:Messages.SequenceID,
+                               view:nat,
+                               operationWrapper:Messages.OperationWrapper) {
+    && v.WF(c)
+    && |ReplicasThatCanCommitInView(c, v, seqID, view, operationWrapper)| < c.clusterConfig.AgreementQuorum()
+  }
+
+  // UnCommitable agrees with Prepares.
+  predicate {:opaque} UnCommitableAgreesWithPrepare(c:Constants, v:Variables) {
+    && v.WF(c)
+    && (forall prepareMsg:Message,
+               priorView:nat,
+               priorOperationWrapper:Messages.OperationWrapper
+                    | && prepareMsg.payload.Prepare? 
+                      && priorView < prepareMsg.payload.view
+                      && c.clusterConfig.IsHonestReplica(prepareMsg.sender)
+                      && priorOperationWrapper != prepareMsg.payload.operationWrapper
+                      && prepareMsg in v.network.sentMsgs
+                         :: UnCommitableInView(c, v, prepareMsg.payload.seqID, priorView, priorOperationWrapper))
+  }
+
+//TODO: write a predicate Prepare matches Commit
+  lemma GetPrepareFromHonestSenderForCommit(c:Constants, v:Variables, commitMsg:Message)
+    returns (prepare:Message)
+    requires Inv(c, v)
+    requires commitMsg.payload.Commit?
+    requires commitMsg in v.network.sentMsgs
+    requires c.clusterConfig.IsHonestReplica(commitMsg.sender)
+    ensures prepare.payload.Prepare?
+    ensures c.clusterConfig.IsHonestReplica(prepare.sender)
+    ensures prepare in v.network.sentMsgs
+    ensures prepare.payload.view == commitMsg.payload.view
+    ensures prepare.payload.seqID == commitMsg.payload.seqID
+    ensures prepare.payload.operationWrapper == commitMsg.payload.operationWrapper
+  {
+    reveal_EveryCommitMsgIsSupportedByAQuorumOfPrepares();
+    var prepares := sentPreparesForSeqID(c, v, commitMsg.payload.view, commitMsg.payload.seqID, commitMsg.payload.operationWrapper);
+    prepare := GetMsgFromHonestSender(c, v, prepares);
+  }
+
+  function FaultyReplicas(c: Constants) : (faulty:set<HostId>) 
+    requires c.WF()
+  {
+    set sender | 0 <= sender < c.clusterConfig.N() && !IsHonestReplica(c, sender)
+  }
+
+  lemma CountFaultyReplicas(c: Constants)
+    requires c.WF()
+    ensures |FaultyReplicas(c)| <= c.clusterConfig.F()
+  {
+    var count := 0;
+    var f := c.clusterConfig.F();
+    var n := c.clusterConfig.N();
+    while(count < n)
+      invariant count <= n
+      invariant |set sender | 0 <= sender < count && !IsHonestReplica(c, sender)| == if count <= f then count
+                                                                                      else f
+      {
+        var oldSet := set sender | 0 <= sender < count && !IsHonestReplica(c, sender);
+        var newSet := set sender | 0 <= sender < count + 1 && !IsHonestReplica(c, sender);
+        if(count + 1 <= f) {
+          assert newSet == oldSet + {count};
+        } else {
+          assert newSet == oldSet;
+        }
+        count := count + 1;
+      }
+  }
+
+  lemma FindHonestNode(c: Constants, replicas:set<HostIdentifiers.HostId>) 
+    returns (honest:HostIdentifiers.HostId)
+    requires c.WF()
+    requires |replicas| >= c.clusterConfig.ByzantineSafeQuorum()
+    requires replicas <= getAllReplicas(c)
+    ensures IsHonestReplica(c, honest)
+    ensures honest in replicas
+  {
+    var honestReplicas := replicas * HonestReplicas(c);
+    CountFaultyReplicas(c);
+    if(|honestReplicas| == 0) {
+      Library.SubsetCardinality(replicas, FaultyReplicas(c));
+      assert false; //Proof by contradiction
+    }
+
+    var result :| result in honestReplicas;
+    honest := result;
+  }
+
+  lemma GetMsgFromHonestSender(c:Constants, v:Variables, quorum:set<Message>)
+    returns (message:Message)
+    requires Inv(c, v)
+    requires |Messages.sendersOf(quorum)| >= c.clusterConfig.AgreementQuorum()
+    requires Messages.sendersOf(quorum) <= getAllReplicas(c)
+    ensures c.clusterConfig.IsHonestReplica(message.sender)
+    ensures message in quorum
+  {
+    var senders := Messages.sendersOf(quorum);
+    var honestSender := FindHonestNode(c, senders);
+    var honest :| honest in quorum && honest.sender == honestSender;
+    message := honest;
+  }
+
+  lemma FindHonestCommitInQuorum(c:Constants,
+                      v:Variables,
+                      seqID:Messages.SequenceID,
+                      view:nat,
+                      commits:set<Message>,
+                      operationWrapper:Messages.OperationWrapper)
+        returns (honestCommit:Message)
+    requires Inv(c, v)
+    requires isCommitQuorum(c, v, view, seqID, operationWrapper, commits)
+    ensures honestCommit in commits
+    ensures IsHonestReplica(c, honestCommit.sender)
+  {
+    var senders := Messages.sendersOf(commits);
+    UniqueSendersCardinality(commits);
+    var honestSender := FindHonestNode(c, senders);
+    var honest :| honest in commits && honest.sender == honestSender;
+    honestCommit := honest;
+  }
+
+  lemma CommitQuorumAgree(c:Constants, v:Variables)
+    requires Inv(c, v)
+    ensures CommitQuorumsAgreeOnOperation(c, v)
+  {
+    forall seqID:Messages.SequenceID,
+           view1:nat,
+           view2:nat,
+           commits1:set<Message>,
+           commits2:set<Message>,
+           operationWrapper1:Messages.OperationWrapper,
+           operationWrapper2:Messages.OperationWrapper
+                | && isCommitQuorum(c, v, view1, seqID, operationWrapper1, commits1)
+                  && isCommitQuorum(c, v, view2, seqID, operationWrapper2, commits2)
+    ensures (operationWrapper1 == operationWrapper2) {
+      if view1 == view2 {
+        // var honestCommit1 := FindHonestCommitInQuorum();
+        var commit1 := FindHonestCommitInQuorum(c, v, seqID, view1, commits1, operationWrapper1);
+        var commit2 := FindHonestCommitInQuorum(c, v, seqID, view2, commits2, operationWrapper2);
+        assert commit1 in v.network.sentMsgs; // Trigger for CommitMsgsFromHonestSendersAgree
+        assert commit2 in v.network.sentMsgs; // Trigger for CommitMsgsFromHonestSendersAgree
+        reveal_CommitMsgsFromHonestSendersAgree();
+        assert commit1.payload.operationWrapper == commit2.payload.operationWrapper;
+        assert operationWrapper1 == operationWrapper2;
+      } else if view1 < view2 {
+        CommitQuorumAgreeDifferentViews(c, v, seqID, view1, view2, commits1, commits2, operationWrapper1, operationWrapper2);
+      } else {
+        CommitQuorumAgreeDifferentViews(c, v, seqID, view2, view1, commits2, commits1, operationWrapper2, operationWrapper1);
+      }
+    }
+  }
+
+  lemma CommitQuorumAgreeDifferentViews(c:Constants, v:Variables,seqID:Messages.SequenceID,
+           view1:nat,
+           view2:nat,
+           commits1:set<Message>,
+           commits2:set<Message>,
+           operationWrapper1:Messages.OperationWrapper,
+           operationWrapper2:Messages.OperationWrapper)
+    requires Inv(c, v)
+    requires isCommitQuorum(c, v, view1, seqID, operationWrapper1, commits1)
+    requires isCommitQuorum(c, v, view2, seqID, operationWrapper2, commits2)
+    requires view1 < view2
+    ensures (operationWrapper1 == operationWrapper2)
+  {
+    reveal_UnCommitableAgreesWithPrepare();
+    if operationWrapper1 != operationWrapper2 {
+      UniqueSendersCardinality(commits2);
+      var commit := GetMsgFromHonestSender(c, v, commits2);
+      var prepare := GetPrepareFromHonestSenderForCommit(c, v, commit); // This term instantiates UnCommitableAgreesWithPrepare
+      UniqueSendersCardinality(commits1);
+      Library.SubsetCardinality(Messages.sendersOf(commits1), ReplicasThatCanCommitInView(c, v, seqID, view1, operationWrapper1));
+      assert !UnCommitableInView(c, v, seqID, view1, operationWrapper1); // We have proven both UnCommitableInView !UnCommitableInView
+      assert false; //proof by contradiction
+    }
+  }
+
+  // Quorum of commits >= 2F+1 agree on all views
+  predicate CommitQuorumsAgreeOnOperation(c:Constants, v:Variables) {
+    && v.WF(c)
+    && (forall seqID:Messages.SequenceID,
+               view1:nat,
+               view2:nat,
+               commits1:set<Message>,
+               commits2:set<Message>,
+               operationWrapper1:Messages.OperationWrapper,
+               operationWrapper2:Messages.OperationWrapper
+                    | && isCommitQuorum(c, v, view1, seqID, operationWrapper1, commits1)
+                      && isCommitQuorum(c, v, view2, seqID, operationWrapper2, commits2)
+                         :: operationWrapper1 == operationWrapper2)
+  }
+
+  predicate HonestReplicasAgreeOnOperationsOrdering(c:Constants, v:Variables) {
+    && v.WF(c)
+    && (forall replica1:HostId, 
+               replica2:HostId,
+               seqID:Messages.SequenceID | && IsHonestReplica(c, replica1)
+                                           && IsHonestReplica(c, replica2)
+                              :: && var r1_c := c.hosts[replica1].replicaConstants;
+                                 && var r2_c := c.hosts[replica2].replicaConstants;
+                                 && var r1_v := v.hosts[replica1].replicaVariables;
+                                 && var r2_v := v.hosts[replica2].replicaVariables;
+                                 && (&& Replica.IsCommitted(r1_c, r1_v, seqID)
+                                     && Replica.IsCommitted(r2_c, r2_v, seqID)) ==> Replica.GetCommittedOperation(r1_c, r1_v, seqID) == Replica.GetCommittedOperation(r2_c, r2_v, seqID))
+
   }
 
   lemma InvariantNext(c: Constants, v:Variables, v':Variables)
@@ -751,6 +1150,15 @@ module Proof {
       HonestPreservesHonestReplicasLockOnCommitForGivenView(c, v, v', step, h_v, h_step);
       HonestPreservesCommitMsgsFromHonestSendersAgree(c, v, v', step, h_v, h_step);
       HonestPreservesRecordedCheckpointsRecvdCameFromNetwork(c, v, v', step, h_v, h_step);
+      //TODO: extract into a lemma.
+      if(h_step.LeaveViewStep?) {
+        HonestLeaveViewStepPreservesUnCommitableAgreesWithPrepare(c, v, v', step, h_v, h_step);
+      } else if(h_step.SendPrepareStep?) {
+        HonestSendPrepareStepPreservesUnCommitableAgreesWithPrepare(c, v, v', step, h_v, h_step);
+      } else {
+        TriviallyPreserveUnCommitableAgreesWithPrepare(c, v, v', step, h_v, h_step);
+      }
+      //END
     } else {
       InvNextFaultyOrClient(c, v, v', step);
     }
@@ -814,6 +1222,12 @@ module Proof {
     assert EveryCommitMsgIsSupportedByAQuorumOfPrepares(c, v') by {
       AlwaysPreservesEveryCommitMsgIsSupportedByAQuorumOfPrepares(c, v, v', step);
     }
+    assert UnCommitableAgreesWithPrepare(c, v') by {
+      var h_step :| true;
+      var h_v :| true;
+      TriviallyPreserveUnCommitableAgreesWithPrepare(c, v, v', step, h_v, h_step);
+    }
+    
   }
 
   lemma InvariantInductive(c: Constants, v:Variables, v':Variables)
